more

Weidenbach_Book/IsaSAT_Backtrack.thy
@@ -2317,13 +2317,6 @@ prepare_code_thms (in -) propagate_bt_wl_D_code_def
 lemmas propagate_bt_wl_D_heur_hnr[sepref_fr_rules] =
   propagate_bt_wl_D_code.refine[OF isasat_input_bounded_nempty_axioms]
 
-text \<open>
-  The difference between \<^term>\<open>isasat_assn\<close> and \<^term>\<open>isasat_fast_assn\<close> corresponds to the
-  following condition:
-\<close>
-abbreviation (in -) isasat_fast :: \<open>twl_st_wl_heur \<Rightarrow> bool\<close> where
-  \<open>isasat_fast S \<equiv> (\<forall>L \<in># dom_m (get_clauses_wl_heur S). L < uint32_max)\<close>
-
 sepref_thm propagate_bt_wl_D_fast_code
   is \<open>uncurry2 (PR_CONST propagate_bt_wl_D_heur)\<close>
   :: \<open>[\<lambda>((L, C), S). isasat_fast S]\<^sub>a
